kami-rv32im: fixed invariants/correctness proofs of fetcher and decoder.

Kami/Ex/ProcFCorrect.v
@@ -6,7 +6,7 @@ Require Import Kami.Renaming Kami.Inline Kami.InlineFacts.
 Require Import Kami.Decomposition Kami.Notations Kami.Tactics.
 Require Import Ex.MemTypes Ex.NativeFifo Ex.MemAsync.
 Require Import Ex.SC Ex.ProcDec Ex.ProcThreeStage Ex.ProcFetch Ex.ProcFInl
-        Ex.ProcFetchDecode.
+        Ex.ProcFInv Ex.ProcFetchDecode.
 Require Import Eqdep.
 
 Set Implicit Arguments.
@@ -37,30 +37,116 @@ Section Fetch.
     (f2dEpoch: forall ty, fullType ty (SyntaxKind f2dElt) ->
                           Expr ty (SyntaxKind Bool)).
 
-  Hypotheses (Hf2dRawInst: forall rawInst curPc nextPc epoch,
-                 evalExpr (f2dRawInst _ (evalExpr (f2dPack rawInst curPc nextPc epoch))) =
-                 evalExpr rawInst)
-             (Hf2dCurPc: forall rawInst curPc nextPc epoch,
-                 evalExpr (f2dCurPc _ (evalExpr (f2dPack rawInst curPc nextPc epoch))) =
-                 evalExpr curPc)
-             (Hf2dNextPc: forall rawInst curPc nextPc epoch,
-                 evalExpr (f2dNextPc _ (evalExpr (f2dPack rawInst curPc nextPc epoch))) =
-                 evalExpr nextPc)
-             (Hf2dEpoch: forall rawInst curPc nextPc epoch,
-                 evalExpr (f2dEpoch _ (evalExpr (f2dPack rawInst curPc nextPc epoch))) =
-                 evalExpr epoch).
-
+  Hypothesis
+    (Hf2dpackExt:
+       forall rawInst1 curPc1 nextPc1 epoch1 rawInst2 curPc2 nextPc2 epoch2,
+         evalExpr rawInst1 = evalExpr rawInst2 ->
+         evalExpr curPc1 = evalExpr curPc2 ->
+         evalExpr nextPc1 = evalExpr nextPc2 ->
+         evalExpr epoch1 = evalExpr epoch2 ->
+         evalExpr (f2dPack rawInst1 curPc1 nextPc1 epoch1) =
+         evalExpr (f2dPack rawInst2 curPc2 nextPc2 epoch2)).
+    
   Variables (pcInit : ConstT (Pc iaddrSize)).
 
   Definition fetchICache: Modules :=
     fetchICache fetch predictNextPc f2dPack pcInit.
+  Definition fetchICacheInl :=
+    ProcFInl.fetchICacheInl fetch predictNextPc f2dPack pcInit.
   Definition fetcher: Modules :=
     ProcFetchDecode.fetcher fetch predictNextPc f2dPack pcInit.
 
+  Definition fetchICache_ruleMap (o: RegsT): string -> option string :=
+    "pgmInitRq" |-> "pgmInitRq";
+      "pgmInitRqEnd" |-> "pgmInitRqEnd";
+      "pgmInitRs" |-> "pgmInitRs";
+      "pgmInitRsEnd" |-> "pgmInitRsEnd";
+      "modifyPc" |-> "modifyPc";
+      "instFetchRs" |-> "instFetch"; ||.
+  Hint Unfold fetchICache_ruleMap: MethDefs.
+
+  Definition fetchICache_regMap (r: RegsT): RegsT :=
+    (mlet pcv : (Pc iaddrSize) <- r |> "pc";
+       mlet pinitv : Bool <- r |> "pinit";
+       mlet pinitRqv : Bool <- r |> "pinitRq";
+       mlet pinitRqOfsv : (Bit iaddrSize) <- r |> "pinitRqOfs";
+       mlet pinitRsOfsv : (Bit iaddrSize) <- r |> "pinitRsOfs";
+       mlet fepochv : Bool <- r |> "fEpoch";
+       mlet bramv : (Vector (Data instBytes) iaddrSize) <- r |> "pgm"--"bram";
+       (["fEpoch" <- existT _ _ fepochv]
+        +["pgm" <- existT _ _ bramv]
+        +["pinitRsOfs" <- existT _ _ pinitRsOfsv]
+        +["pinitRqOfs" <- existT _ _ pinitRqOfsv]
+        +["pinitRq" <- existT _ _ pinitRqv]
+        +["pinit" <- existT _ _ pinitv]
+        +["pc" <- existT _ _ pcv]
+       )%fmap)%mapping.
+  Hint Unfold fetchICache_regMap: MapDefs.
+
+  Ltac fetchICache_dest_tac :=
+    repeat match goal with
+           | [H: context[fetchICache_inv] |- _] => destruct H
+           end;
+    kinv_red.
+
   Theorem fetchICache_refines_fetcher:
     fetchICache <<== fetcher.
-  Proof.
-  Admitted.
+  Proof. (* SKIP_PROOF_OFF *)
+
+    (** inlining *)
+    ketrans; [exact (projT2 fetchICacheInl)|].
+
+    (** decomposition *)
+    kdecompose_nodefs fetchICache_regMap fetchICache_ruleMap.
+    kinv_add fetchICache_inv_ok.
+    kinv_add_end.
+    kinvert.
+
+    - kinv_action_dest.
+      kinv_custom fetchICache_dest_tac.
+      kinv_regmap_red.
+      kinv_constr; kinv_eq; kinv_finish.
+
+    - kinv_action_dest.
+      kinv_custom fetchICache_dest_tac.
+      kinv_regmap_red.
+      kinv_constr; kinv_eq; kinv_finish.
+
+    - kinv_action_dest.
+      kinv_custom fetchICache_dest_tac.
+      kinv_regmap_red.
+      kinv_constr; kinv_eq; kinv_finish.
+
+    - kinv_action_dest.
+      kinv_custom fetchICache_dest_tac.
+      kinv_regmap_red.
+      kinv_constr; kinv_eq; kinv_finish.
+
+    - kinv_action_dest.
+      kinv_custom fetchICache_dest_tac.
+      kinv_regmap_red.
+      kinv_constr; kinv_eq.
+
+    - kinv_action_dest.
+      kinv_custom fetchICache_dest_tac.
+      kinv_regmap_red.
+      kinv_constr; kinv_eq.
+
+    - kinv_action_dest.
+      kinv_custom fetchICache_dest_tac.
+      kinv_regmap_red.
+      kinv_constr; kinv_eq.
+      apply Hf2dpackExt; try reflexivity.
+      simpl.
+      destruct x0; [subst|discriminate].
+      reflexivity.
+
+    - kinv_action_dest.
+      kinv_custom fetchICache_dest_tac.
+      kinv_regmap_red.
+      kinv_constr; kinv_eq.
+      (* END_SKIP_PROOF_OFF *)
+  Qed.
 
 End Fetch.
 
