Kami/Ex/ProcFDCorrect.v
@@ -63,7 +63,15 @@ Section FetchDecode.
                  evalExpr nextPc)
              (Hf2dEpoch: forall rawInst curPc nextPc epoch,
                  evalExpr (f2dEpoch _ (evalExpr (f2dPack rawInst curPc nextPc epoch))) =
-                 evalExpr epoch).
+                 evalExpr epoch)
+             (Hf2dpackExt:
+                forall rawInst1 curPc1 nextPc1 epoch1 rawInst2 curPc2 nextPc2 epoch2,
+                  evalExpr rawInst1 = evalExpr rawInst2 ->
+                  evalExpr curPc1 = evalExpr curPc2 ->
+                  evalExpr nextPc1 = evalExpr nextPc2 ->
+                  evalExpr epoch1 = evalExpr epoch2 ->
+                  evalExpr (f2dPack rawInst1 curPc1 nextPc1 epoch1) =
+                  evalExpr (f2dPack rawInst2 curPc2 nextPc2 epoch2)).
 
   Variables (pcInit : ConstT (Pc iaddrSize)).
 
@@ -83,7 +91,11 @@ Section FetchDecode.
   Hint Extern 1 (ModEquiv type typeUT fetchNDecode) => unfold fetchNDecode. (* for kequiv *)
 
   Definition fetchDecode_ruleMap (o: RegsT): string -> option string :=
-    "modifyPc" |-> "modifyPc";
+    "pgmInitRq" |-> "pgmInitRq";
+      "pgmInitRqEnd" |-> "pgmInitRqEnd";
+      "pgmInitRs" |-> "pgmInitRs";
+      "pgmInitRsEnd" |-> "pgmInitRsEnd";
+      "modifyPc" |-> "modifyPc";
       "decodeLd" |-> "instFetchLd";
       "decodeSt" |-> "instFetchSt";
       "decodeTh" |-> "instFetchTh";
@@ -92,13 +104,20 @@ Section FetchDecode.
 
   Definition fetchDecode_regMap (r: RegsT): RegsT :=
     (mlet pcv : (Pc iaddrSize) <- r |> "pc";
+       mlet pinitv : Bool <- r |> "pinit";
+       mlet pinitRqv : Bool <- r |> "pinitRq";
+       mlet pinitRqOfsv : (Bit iaddrSize) <- r |> "pinitRqOfs";
+       mlet pinitRsOfsv : (Bit iaddrSize) <- r |> "pinitRsOfs";
        mlet pgmv : (Vector (Data instBytes) iaddrSize) <- r |> "pgm";
        mlet fev : Bool <- r |> "fEpoch";
        mlet f2dfullv : Bool <- r |> "f2d"--"full";
        mlet f2deltv : f2dElt <- r |> "f2d"--"elt";
-
        (["fEpoch" <- existT _ _ fev]
         +["pgm" <- existT _ _ pgmv]
+        +["pinitRsOfs" <- existT _ _ pinitRsOfsv]
+        +["pinitRqOfs" <- existT _ _ pinitRqOfsv]
+        +["pinitRq" <- existT _ _ pinitRqv]
+        +["pinit" <- existT _ _ pinitv]
         +["pc" <- existT _ (SyntaxKind (Pc iaddrSize))
                (if f2dfullv then evalExpr (f2dCurPc _ f2deltv)
                 else pcv)])%fmap)%mapping.
@@ -113,7 +132,12 @@ Section FetchDecode.
     try rewrite Hf2dRawInst in *;
     try rewrite Hf2dCurPc in *;
     try rewrite Hf2dNextPc in *;
-    try rewrite Hf2dEpoch in *.
+    try rewrite Hf2dEpoch in *;
+    repeat
+      match goal with
+      | [H: ?pinitv = false -> true = false |- ?pinitv = true] =>
+        destruct pinitv; [reflexivity|specialize (H eq_refl); discriminate]
+      end.
 
   Ltac fetchDecode_dest_tac :=
     repeat match goal with
@@ -129,9 +153,28 @@ Section FetchDecode.
 
   Theorem fetchDecode_refines_fetchNDecode:
     fetchDecode <<== fetchNDecode.
-  Proof. (* SKIP_PROOF_ON
-    kami_ok fdConfig fetchDecode_dest_tac f2d_abs_tac.
-    END_SKIP_PROOF_ON *) apply cheat.
+  Proof. (* SKIP_PROOF_OFF *)
+
+    (** inlining *)
+    ketrans; [exact (projT2 fetchDecodeInl)|].
+
+    (** decomposition *)
+    kdecompose_nodefs fetchDecode_regMap fetchDecode_ruleMap.
+    kinv_add fetchDecode_inv_ok.
+    kinv_add_end.
+    kinvert.
+    - kinv_magic_with fetchDecode_dest_tac f2d_abs_tac.
+    - kinv_magic_with fetchDecode_dest_tac f2d_abs_tac.
+    - kinv_magic_with fetchDecode_dest_tac f2d_abs_tac.
+    - kinv_magic_with fetchDecode_dest_tac f2d_abs_tac.
+    - kinv_magic_with fetchDecode_dest_tac f2d_abs_tac.
+    - kinv_magic_with fetchDecode_dest_tac f2d_abs_tac.
+    - kinv_magic_with fetchDecode_dest_tac f2d_abs_tac.
+    - kinv_magic_with fetchDecode_dest_tac f2d_abs_tac.
+    - kinv_magic_with fetchDecode_dest_tac f2d_abs_tac.
+    
+      (* kami_ok fdConfig fetchDecode_dest_tac f2d_abs_tac. *)
+      (* END_SKIP_PROOF_OFF *)
   Qed.
 
   Theorem fetchICacheDecode_refines_fetchDecode:
